quick and incomplete support for accessing single-field records

LiveVerif/src/LiveVerifExamples/swap_record_fields.v
@@ -9,15 +9,29 @@ Record foo := {
   fieldD: Z;
 }.
 
+Record singleton_foo := {
+  singleField: Z;
+}.
+
 Load LiveVerif.
 
 Definition foo_t(r: foo): word -> mem -> Prop := .**/
+
 typedef struct __attribute__ ((__packed__)) {
   uint32_t fieldA;
   uint32_t fieldB;
   uint32_t fieldC;
   uint32_t fieldD;
 } foo_t;
+
+/**.
+
+Definition singleton_foo_t(r: singleton_foo): word -> mem -> Prop := .**/
+
+typedef struct __attribute__ ((__packed__)) {
+  uint32_t singleField;
+} singleton_foo_t;
+
 /**.
 
 #[export] Instance spec_of_swap_bc: fnspec :=                                   .**/
@@ -35,6 +49,31 @@ Derive swap_bc SuchThat (fun_correct! swap_bc) As swap_bc_ok.                   
 } /**.
 reflexivity. (* TODO automate, but don't use reflexivity in the library, because
   especially on unprovable goals with evars, it can run forever *)
+Qed.
+
+#[export] Instance spec_of_swap_singleField: fnspec :=                          .**/
+
+void swap_singleField(uintptr_t p, uintptr_t q) /**#
+  ghost_args := f1 f2 (R: mem -> Prop);
+  requires t m := <{ * singleton_foo_t f1 p
+                     * singleton_foo_t f2 q
+                     * R }> m;
+  ensures t' m' := t' = t /\
+       <{ * singleton_foo_t {| singleField := singleField f1 |} q
+          * singleton_foo_t {| singleField := singleField f2 |} p
+          * R }> m'
+       (* TODO also prove the following postcondition automatically:
+       <{ * uint 32 (singleField f2) p
+          * uint 32 (singleField f1) q
+          * R }> m'
+       <{ * singleton_foo_t f2 p
+          * singleton_foo_t f1 q
+          * R }> m' *) #**/                                                 /**.
+Derive swap_singleField SuchThat (fun_correct! swap_singleField) As
+  swap_singleField_ok.                                                          .**/
+{                                                                          /**. .**/
+  swap(p, q);                                                              /**. .**/
+} /**.
 Qed.
 
   (* TODO: example where a loop uses a pointer to an element of an array inside a record
